src/Bytes.v
@@ -1,0 +1,62 @@
+Require Import Word.
+Require Import Arith.
+Require Import Eqdep_dec.
+
+Set Implicit Arguments.
+
+Definition byte := word 8.
+Definition bytes n := word (n * 8).
+
+Definition word2bytes nbits nbytes (H : nbits = nbytes * 8) (w : word nbits) : bytes nbytes :=
+  eq_rect nbits word w (nbytes*8) H.
+
+Definition bcombine (sz1 : nat) (bs1 : bytes sz1) (sz2 : nat) (bs2 : bytes sz2) : bytes (sz1 + sz2).
+  unfold bytes in *.
+  rewrite Nat.mul_add_distr_r in *.
+  exact (combine bs1 bs2).
+Defined.
+
+Definition bsplit1 (sz1 sz2 : nat) (bs : bytes (sz1 + sz2)) : bytes sz1.
+  unfold bytes in *.
+  rewrite Nat.mul_add_distr_r in *.
+  exact (split1 _ _ bs).
+Defined.
+
+Definition bsplit2 (sz1 sz2 : nat) (bs : bytes (sz1 + sz2)) : bytes sz2.
+  unfold bytes in *.
+  rewrite Nat.mul_add_distr_r in *.
+  exact (split2 _ _ bs).
+Defined.
+
+Hint Rewrite combine_split : bytehints.
+Hint Rewrite split1_combine : bytehints.
+Hint Rewrite split2_combine : bytehints.
+Hint Rewrite eq_rect_nat_double : bytehints.
+Hint Rewrite <- (eq_rect_eq_dec eq_nat_dec) : bytehints.
+
+Theorem bcombine_bsplit : forall sz1 sz2 (bs : bytes (sz1 + sz2)),
+  bcombine (bsplit1 sz1 sz2 bs) (bsplit2 sz1 sz2 bs) = bs.
+Proof.
+  unfold bcombine, bsplit1, bsplit2, eq_rec_r, eq_rec.
+  intros.
+  autorewrite with bytehints.
+  reflexivity.
+Qed.
+
+Theorem bsplit1_bcombine : forall sz1 sz2 (bs : bytes sz1) (z : bytes sz2),
+  bsplit1 sz1 sz2 (bcombine bs z) = bs.
+Proof.
+  unfold bcombine, bsplit1, bsplit2, eq_rec_r, eq_rec.
+  intros.
+  autorewrite with bytehints.
+  reflexivity.
+Qed.
+
+Theorem bsplit2_bcombine : forall sz1 sz2 (bs : bytes sz1) (z : bytes sz2),
+  bsplit2 sz1 sz2 (bcombine bs z) = z.
+Proof.
+  unfold bcombine, bsplit1, bsplit2, eq_rec_r, eq_rec.
+  intros.
+  autorewrite with bytehints.
+  reflexivity.
+Qed.
